countable formulae, and trying extend/insert/delta/max approach for lindenbaum

PdlParallelStoring/Completeness.lean
@@ -1,29 +1,16 @@
 import Mathlib.Data.Finset.Basic
+import Mathlib.Data.Set.Lattice
 
 import PdlParallelStoring.AxiomaticSystem
 import PdlParallelStoring.Properties
+
+open Classical
 
 -- Predicates for formulae and programs in the RSPDL₀ fragment.
 -- In this fragment, we do not allow the use of the operators of:
 --   - test (?)
 --   - iteration (★)
 --   - parallel composition (‖).
-
-inductive RSPDL0Program : π → Prop where
-  | atomic α : RSPDL0Program (π.atomic α)
-  | comp α β : RSPDL0Program α → RSPDL0Program β → RSPDL0Program (α ; β)
-  | choice α β : RSPDL0Program α → RSPDL0Program β → RSPDL0Program (α ∪ β)
-  | s₁ : RSPDL0Program π.s₁
-  | s₂ : RSPDL0Program π.s₂
-  | r₁ : RSPDL0Program π.r₁
-  | r₂ : RSPDL0Program π.r₂
-
-inductive RSPDL0Formula : Φ → Prop where
-  | false : RSPDL0Formula ⊥'
-  | atomic φ : RSPDL0Formula (Φ.atomic φ)
-  | neg φ : RSPDL0Formula φ → RSPDL0Formula (¬ φ)
-  | conj φ₁ φ₂ : RSPDL0Formula φ₁ → RSPDL0Formula φ₂ → RSPDL0Formula (φ₁ ∧ φ₂)
-  | diamond π φ : RSPDL0Program π → RSPDL0Formula φ → RSPDL0Formula (⟨π⟩ φ)
 
 def listToConjunction : List Φ → Φ
   | [] => ⊤'
@@ -34,19 +21,16 @@ noncomputable def finsetToConjunction (φs : Finset Φ) : Φ :=
   listToConjunction φs.toList
 
 def IsConsistent (s : Set Φ) : Prop :=
-  (∀ φ ∈ s, RSPDL0Formula φ) ∧
   ¬ ∃ (φs : Finset Φ), (∀ φ ∈ φs, φ ∈ s) ∧ (⊢ (finsetToConjunction φs → ⊥'))
 
 lemma consistent_empty : IsConsistent ∅ := by
   sorry
 
-lemma deduction_consistency (φ : Φ) : RSPDL0Formula φ → ((⊢ φ) ↔ ¬ IsConsistent {¬ φ}) := by
-  intro hRSPDL0
+lemma deduction_consistency (φ : Φ) : ((⊢ φ) ↔ ¬ IsConsistent {¬ φ}) := by
   constructor
   · intros hProv
     rewrite [IsConsistent]
     push_neg
-    intros _
     use {¬ φ}
     constructor
     · simp
@@ -61,11 +45,7 @@ lemma deduction_consistency (φ : Φ) : RSPDL0Formula φ → ((⊢ φ) ↔ ¬ Is
     by_contra hInconsistent
     rewrite [IsConsistent] at hInconsistent
     push_neg at hInconsistent
-    obtain ⟨φ₂s, hSubset, hDerivesFalse⟩ := hInconsistent (by
-      intros φ₂ hφ₂In
-      simp only [Set.mem_singleton_iff] at hφ₂In
-      rewrite [hφ₂In]
-      exact RSPDL0Formula.neg φ hRSPDL0)
+    obtain ⟨φ₂s, hSubset, hDerivesFalse⟩ := hInconsistent
     by_cases hEmpty : φ₂s = ∅
     case pos =>
       rewrite [hEmpty] at hDerivesFalse
@@ -106,28 +86,77 @@ lemma deduction_consistency (φ : Φ) : RSPDL0Formula φ → ((⊢ φ) ↔ ¬ Is
       have hProv : ⊢ φ := RSPDL₀.classicalNegation φ hDerivesFalse
       exact hNotProv hProv
 
-lemma unprovable_consistent (φ : Φ) : RSPDL0Formula φ → (¬ ⊢ φ) → IsConsistent {¬ φ} := by
-  intros hRPSDL0 hNotProv
-  rewrite [deduction_consistency φ hRPSDL0] at hNotProv
+lemma unprovable_consistent (φ : Φ) : (¬ ⊢ φ) → IsConsistent {¬ φ} := by
+  intros hNotProv
+  rewrite [deduction_consistency φ] at hNotProv
   exact Classical.not_not.mp hNotProv
 
 def IsMaximal (s : Set Φ) : Prop :=
   IsConsistent s ∧
-  ∀ {φ : Φ}, RSPDL0Formula φ → (φ ∉ s) → ¬ IsConsistent (s ∪ {φ})
+  ∀ {φ : Φ}, (φ ∉ s) → ¬ IsConsistent (s ∪ {φ})
 
 def MaximalConsistentSet : Type :=
   {s : Set Φ // IsMaximal s}
 
-lemma mcs_complete (Γ : MaximalConsistentSet) (φ : Φ) :
-  RSPDL0Formula φ → (φ ∈ Γ.val) ∨ (¬ φ) ∈ Γ.val := by
+lemma mcs_complete (Γ : MaximalConsistentSet) (φ : Φ) : (φ ∈ Γ.val) ∨ (¬ φ) ∈ Γ.val := by
   sorry
 
-lemma mcs_no_contradiction (Γ : MaximalConsistentSet) (φ : Φ) :
-  RSPDL0Formula φ → (φ ∈ Γ.val) → (¬ φ) ∉ Γ.val := by
+lemma mcs_no_contradiction (Γ : MaximalConsistentSet) (φ : Φ) : (φ ∈ Γ.val) → (¬ φ) ∉ Γ.val := by
   sorry
 
-lemma lindenbaum (s : Set Φ) : IsConsistent s → ∃ (Γ : MaximalConsistentSet), s ⊆ Γ.val := by
+namespace Lindenbaum
+
+def extend (φ : Φ) (Γ : Set Φ) : Set Φ :=
+  Γ ∪ {φ}
+
+noncomputable def insert : Option Φ → Set Φ → Set Φ
+  | none, Γ => Γ
+  | some φ, Γ =>
+      if IsConsistent (extend φ Γ)
+      then extend φ Γ
+      else extend (¬ φ) Γ
+
+def delta (Γ : Set Φ) : Nat → Set Φ
+  | 0 => Γ
+  | n + 1 => insert (decode n) (delta Γ n)
+
+def max (Γ : Set Φ) : Set Φ :=
+  ⋃ n, delta Γ n
+
+lemma consistency_either (Γ : Set Φ) (φ : Φ) :
+    IsConsistent Γ →
+    IsConsistent (extend φ Γ) ∨ IsConsistent (extend (¬ φ) Γ) := by
   sorry
+
+lemma insert_preserves_consistency (opt_φ : Option Φ) (Γ : Set Φ) :
+    IsConsistent Γ → IsConsistent (insert opt_φ Γ) := by
+  intros hConsistent
+  cases opt_φ with
+  | none => exact hConsistent
+  | some φ =>
+      simp [insert]
+      split_ifs with h
+      . exact h
+      . have hEither := consistency_either Γ φ hConsistent
+        cases hEither with
+        | inl _ => contradiction
+        | inr hRight => exact hRight
+
+lemma delta_preserves_consistency (Γ : Set Φ) (n : Nat) :
+    IsConsistent Γ → IsConsistent (delta Γ n) := by
+  intros hConsistent
+  induction n with
+  | zero => exact hConsistent
+  | succ n ih =>
+      apply insert_preserves_consistency
+      exact ih
+
+lemma lindenbaum (Γ : Set Φ) : IsConsistent Γ → ∃ (Δ : MaximalConsistentSet), Γ ⊆ Δ.val := by
+  /- intros hConsistent -/
+  /- exists (max Γ) -/
+  sorry
+
+end Lindenbaum
 
 def canonicalRelation (α : π) (Γ Δ : MaximalConsistentSet) : Prop :=
   ∀ φ, (([α] φ) ∈ Γ.val) → φ ∈ Δ.val
@@ -144,8 +173,7 @@ def canonicalModel : Model where
   F := canonicalFrame
   V := canonicalValuation
 
-lemma truth_lemma (φ : Φ) (Γ : canonicalModel.F.W) :
-  RSPDL0Formula φ → (((canonicalModel, Γ) ⊨ φ) ↔ φ ∈ Γ.val) := by
+lemma truth_lemma (φ : Φ) (Γ : canonicalModel.F.W) : ((canonicalModel, Γ) ⊨ φ) ↔ φ ∈ Γ.val := by
   sorry
 
 instance canonicalProper : Proper canonicalFrame := by
@@ -159,18 +187,18 @@ instance : ProperStandard canonicalModel where
   toProper := canonicalProper
 
 lemma contrapositive_completeness :
-    ∀ {φ : Φ}, RSPDL0Formula φ → (¬ ⊢ φ) →
+    ∀ {φ : Φ}, (¬ ⊢ φ) →
     ∃ (M : Model) (_ : ProperStandard M), ¬ (M ⊨ φ) := by
-  intro φ hRSPDL0 hNotProv
-  have h₁ : IsConsistent {¬ φ} := unprovable_consistent φ hRSPDL0 hNotProv
-  obtain ⟨Γ, h₂⟩ := lindenbaum {¬ φ} h₁
+  intro φ hNotProv
+  have h₁ : IsConsistent {¬ φ} := unprovable_consistent φ hNotProv
+  obtain ⟨Γ, h₂⟩ := Lindenbaum.lindenbaum {¬ φ} h₁
   have h₃ : (¬ φ) ∈ Γ.val := h₂ (Set.mem_singleton (¬ φ))
   have h₄ : φ ∉ Γ.val := by
     by_contra hIn
-    have hNotIn:= mcs_no_contradiction Γ φ hRSPDL0 hIn
+    have hNotIn:= mcs_no_contradiction Γ φ hIn
     exact hNotIn h₃
   have h₅ : ¬ ((canonicalModel, Γ) ⊨ φ) := by
-    rewrite [truth_lemma φ Γ hRSPDL0]
+    rewrite [truth_lemma φ Γ]
     exact h₄
   use canonicalModel, inferInstance
   intro hGlobalSat
@@ -180,7 +208,6 @@ lemma contrapositive_completeness :
 theorem completeness : ∀ {φ : Φ}, (⊨ φ) → (⊢ φ) := by
   intro φ hValid
   by_contra hNotProv
-  have hRSPDL0 : RSPDL0Formula φ := sorry
-  obtain ⟨M, _, hNotGlobalSat⟩ := contrapositive_completeness hRSPDL0 hNotProv
+  obtain ⟨M, _, hNotGlobalSat⟩ := contrapositive_completeness hNotProv
   have hGlobalSat : M ⊨ φ := hValid rfl
   exact hNotGlobalSat hGlobalSat
